TouhouFormal/ECL.lean
@@ -16,6 +16,7 @@ import TouhouFormal.ECL.Unary
 import TouhouFormal.ECL.FloatFunction
 import TouhouFormal.ECL.Random
 import TouhouFormal.ECL.Movement
+import TouhouFormal.ECL.TimedMovement
 import TouhouFormal.ECL.EnemyState
 import TouhouFormal.ECL.Shooting
 import TouhouFormal.ECL.BulletPattern
